cedar-lean/Cedar/Thm.lean
@@ -18,3 +18,4 @@ import Cedar.Thm.Authorization
 import Cedar.Thm.Partial
 import Cedar.Thm.Slicing
 import Cedar.Thm.Typechecking
+import Cedar.Thm.Entities
