cedar-lean/Cedar/Thm/Entities.lean
@@ -1,0 +1,5 @@
+
+import Batteries.Data.List
+namespace Cedar.Entities
+
+end Cedar.Entities
