cedar-lean/Cedar/Validation/Typechecker.lean
@@ -53,19 +53,15 @@ def typeOfLit (p : Prim) (env : Environment) (inf : Bool) : ResultType :=
     -- Type the entity at level 0 if we're checking a finite leve schema
     --  This will forbid derefernces of entity literals
     -- othewise give it level infinity
-    then ok (.entity {
-      typeName := uid.ty,
-      level := if inf then .infinite else .finite 0
-    })
+    then ok (.entity uid.ty (if inf then Level.infinite else Level.finite 0 ))
     else err (.unknownEntity uid.ty)
 
 def typeOfVar (v : Var) (env : Environment) : ResultType :=
   match v with
-  | .principal => ok (.entity env.reqty.principal)
+  | .principal => ok (.entity env.reqty.principal.fst env.reqty.principal.snd)
   | .action    =>
-    let ety := { typeName := env.reqty.action.fst.ty, level := env.reqty.action.snd }
-    ok (.entity ety)
-  | .resource  => ok (.entity env.reqty.resource)
+    ok (.entity env.reqty.action.fst.ty env.reqty.action.snd)
+  | .resource => ok (.entity env.reqty.resource.fst env.reqty.resource.snd)
   | .context   => ok (.record env.reqty.context)
 
 def typeOfIf (r₁ : CedarType × Capabilities) (r₂ r₃ : ResultType) : ResultType :=
@@ -116,7 +112,7 @@ def typeOfUnaryApp (op : UnaryOp) (ty : CedarType) : ResultType :=
   | .not, .bool x          => ok (.bool x.not)
   | .neg, .int             => ok .int
   | .like _, .string       => ok (.bool .anyBool)
-  | .is ety₁, .entity ety₂ => ok (.bool (if ety₁ = ety₂.typeName then .tt else .ff))
+  | .is ety₁, .entity ety₂ _ => ok (.bool (if ety₁ = ety₂ then .tt else .ff))
   | _, _                   => err (.unexpectedType ty)
 
 def typeOfEq (ty₁ ty₂ : CedarType) (x₁ x₂ : Expr) : ResultType :=
@@ -127,7 +123,7 @@ def typeOfEq (ty₁ ty₂ : CedarType) (x₁ x₂ : Expr) : ResultType :=
     | .some _ => ok (.bool .anyBool)
     | .none   =>
     match ty₁, ty₂ with
-    | .entity _, .entity _ => ok (.bool .ff)
+    | .entity _ _, .entity _ _ => ok (.bool .ff)
     | _, _                 => err (.lubErr ty₁ ty₂)
 
 def entityUID? : Expr → Option EntityUID
@@ -142,29 +138,29 @@ def actionUID? (x : Expr) (acts: ActionSchema) : Option EntityUID := do
   let uid ← entityUID? x
   if acts.contains uid then .some uid else .none
 
--- x₁ in x₂ where x₁ has type ety₁ and x₂ has type ety₂
-def typeOfInₑ (ety₁ ety₂ : LeveledEntityType) (x₁ x₂ : Expr) (env : Environment) : ResultType :=
-  if ety₁.level > .finite 0 then type else err $ .levelError ety₁.typeName
+-- x₁ in x₂ where x₁ has type ety₁ at level l₁ and x₂ has type ety₂
+def typeOfInₑ (ety₁  ety₂ : EntityType) (l₁ : Level ) (x₁ x₂ : Expr) (env : Environment) : ResultType :=
+  if l₁ > Level.zero then ok (.bool type) else err (.levelError ety₁)
   where
-    type := ok $ .bool $ match actionUID? x₁ env.acts, entityUID? x₂ with
-        | .some uid₁, .some uid₂ =>
-          if env.acts.descendentOf uid₁ uid₂
-          then .tt else .ff
-        | _, _ =>
-          if env.ets.descendentOf ety₁.typeName ety₂.typeName
-          then .anyBool else .ff
+    type := match actionUID? x₁ env.acts, entityUID? x₂ with
+            | .some uid₁, .some uid₂ =>
+              if env.acts.descendentOf uid₁ uid₂
+              then .tt else .ff
+            | _, _ =>
+              if env.ets.descendentOf ety₁ ety₂
+              then .anyBool else .ff
 
--- x₁ in x₂ where x₁ has type ety₁ and x₂ has type (.set ety₂)
-def typeOfInₛ (ety₁ ety₂ : LeveledEntityType) (x₁ x₂ : Expr) (env : Environment) : ResultType :=
-  if ety₁.level > .finite 0 then type else err $ .levelError ety₁.typeName
+-- x₁ in x₂ where x₁ has type ety₁ at level l₁ and x₂ has type (.set ety₂)
+def typeOfInₛ (ety₁ ety₂ : EntityType) (l₁ : Level) (x₁ x₂ : Expr) (env : Environment) : ResultType :=
+  if l₁ > Level.zero then ok (.bool type) else err (.levelError ety₁)
   where
-    type := ok $ .bool $  match actionUID? x₁ env.acts, entityUIDs? x₂ with
-        | .some uid₁, .some uids =>
-          if uids.any (env.acts.descendentOf uid₁ ·)
-          then .tt else .ff
-        | _, _ =>
-          if env.ets.descendentOf ety₁.typeName ety₂.typeName
-          then .anyBool else .ff
+    type := match actionUID? x₁ env.acts, entityUIDs? x₂ with
+            | .some uid₁, .some uids =>
+              if uids.any (env.acts.descendentOf uid₁ ·)
+              then .tt else .ff
+            | _, _ =>
+              if env.ets.descendentOf ety₁ ety₂
+              then .anyBool else .ff
 
 def ifLubThenBool (ty₁ ty₂ : CedarType) : ResultType :=
   match ty₁ ⊔ ty₂ with
@@ -174,8 +170,8 @@ def ifLubThenBool (ty₁ ty₂ : CedarType) : ResultType :=
 def typeOfBinaryApp (op₂ : BinaryOp) (ty₁ ty₂ : CedarType) (x₁ x₂ : Expr) (env : Environment) : ResultType :=
   match op₂, ty₁, ty₂ with
   | .eq, _, _                               => typeOfEq ty₁ ty₂ x₁ x₂
-  | .mem, .entity ety₁, .entity ety₂        => (typeOfInₑ ety₁ ety₂ x₁ x₂ env)
-  | .mem, .entity ety₁, .set (.entity ety₂) => (typeOfInₛ ety₁ ety₂ x₁ x₂ env)
+  | .mem, .entity ety₁ l₁, .entity ety₂ _        => (typeOfInₑ ety₁ ety₂ l₁ x₁ x₂ env)
+  | .mem, .entity ety₁ l₁, .set (.entity ety₂ _) => (typeOfInₛ ety₁ ety₂ l₁ x₁ x₂ env)
   | .less,   .int, .int                     => ok (.bool .anyBool)
   | .lessEq, .int, .int                     => ok (.bool .anyBool)
   | .add,    .int, .int                     => ok .int
@@ -200,37 +196,55 @@ def actionType? (ety : EntityType) (acts: ActionSchema) : Bool :=
 def typeOfHasAttr (ty : CedarType) (x : Expr) (a : Attr) (c : Capabilities) (env : Environment) : ResultType :=
   match ty with
   | .record rty => hasAttrInRecord rty x a c true
-  | .entity ety =>
+  | .entity ety level =>
         let hasType :=
-          match env.ets.attrs? ety.typeName  with
+          match env.ets.attrs? ety with
           | .some rty => hasAttrInRecord rty x a c false
           | .none     =>
-            if actionType? ety.typeName env.acts
+            if actionType? ety env.acts
             then ok (.bool .ff) -- action attributes not allowed
-            else err (.unknownEntity ety.typeName)
-        if ety.level > .finite 0 then hasType else err $ .levelError ety.typeName
+            else err (.unknownEntity ety)
+        if level > Level.zero then hasType else err (.levelError ety)
   | _           => err (.unexpectedType ty)
 
-def delevel (cur : Level) (ty : CedarType)  : CedarType :=
+
+def setLevel (l: Level) (ty : CedarType)  : CedarType :=
   match ty with
   | .bool b => .bool b
   | .int => .int
   | .string => .string
-  | .entity ety  => .entity $ ety.setLevel cur.sub1
-  | .set ty => .set $ delevel cur ty
+  | .entity ety l  => .entity ety l
+  | .set ty => .set $ setLevel l ty
   | .record rty =>
-    let kvs := rty.kvs.map₁ (
-      λ pair =>
-        let fst := pair.val.fst
-        let snd := (delevel cur) <$> pair.val.snd
-        (fst, snd)
-    )
-    .record $ Map.mk kvs
+    .record (Map.mk ((List.attach (rty.kvs)).map (λ pair =>
+      let attrName := pair.val.fst
+      let ty := match _h : pair.val.snd with
+                | .required ty => .required (setLevel l ty)
+                | .optional ty => .optional (setLevel l ty)
+      (attrName, ty)
+    )))
   | .ext ty => .ext ty
 termination_by sizeOf ty
 decreasing_by
-  all_goals sorry
-
+  all_goals simp_wf
+  all_goals try omega
+  all_goals {
+      have h₁ : sizeOf ty < sizeOf pair.val.snd := by
+        rw [_h]
+        simp
+        omega
+      have h₂ : sizeOf pair.val.snd < sizeOf pair.val := by
+        cases pair.val
+        case mk fst snd =>
+          simp_wf
+          omega
+      have h₃ : sizeOf rty.kvs < sizeOf rty := by
+        apply Cedar.Data.Map.sizeOf_lt_of_kvs
+      have h₄ : sizeOf pair.val < sizeOf rty.kvs := by
+        apply List.sizeOf_lt_of_mem
+        apply pair.property
+      omega
+  }
 
 
 
@@ -244,14 +258,14 @@ def getAttrInRecord (ty : CedarType) (rty : RecordType) (x : Expr) (a : Attr) (c
 def typeOfGetAttr (ty : CedarType) (x : Expr) (a : Attr) (c : Capabilities) (env : Environment) : ResultType :=
   match ty with
   | .record rty => getAttrInRecord ty rty x a c
-  | .entity ety =>
-    if ety.level > .finite 0 then
-      match env.ets.attrs? ety.typeName with
+  | .entity ety level =>
+    if level > Level.zero then
+      match env.ets.attrs? ety with
       | .some rty => do
         let (type, caps) ← getAttrInRecord ty rty x a c
-        .ok (delevel ety.level type, caps)
-      | .none     => err (.unknownEntity ety.typeName)
-    else err $ .levelError ety.typeName
+        .ok (setLevel level.sub1 type, caps)
+      | .none     => err (.unknownEntity ety)
+    else err $ .levelError ety
   | _           => err (.unexpectedType ty)
 
 def typeOfSet (tys : List CedarType) : ResultType :=
